iris/WpGprMretNew.v
@@ -23,6 +23,7 @@ From iris.proofmode Require Import proofmode.
 From iris.program_logic Require Import language.
 Require Import SailStdpp.Operators_mwords.
 Require Import Riscv.rv64d_types Riscv.rv64d.
+Require Import WpGprCsrwCommon.
 Require Import SailStdpp.Base.
 Require Import RiscvLang RiscvPtsto RiscvExec RiscvTryStep RiscvFetchExec.
 Require Import MinstretInv.
