iris/WpPopOff.v
@@ -29,6 +29,7 @@ From iris.proofmode Require Import proofmode.
 From iris.program_logic Require Import language lifting.
 Require Import SailStdpp.ConcurrencyInterface SailStdpp.ConcurrencyInterfaceBuiltins SailStdpp.ConcurrencyInterfaceTypes SailStdpp.Operators_mwords.
 Require Import Riscv.rv64d_types Riscv.rv64d Riscv.riscv_extras.
+Require Import WpGprCsrwCommon.
 Require Import RiscvModelBytes.
 Require Import SailStdpp.Base SailStdpp.TypeCasts SailStdpp.Values SailStdpp.MachineWord.
 Require Import RiscvLang RiscvPtsto RiscvExec RiscvExtras RiscvTryStep RiscvFetchExec.
