iris/WpStartNew.v
@@ -55,6 +55,7 @@ From iris.base_logic.lib Require Import ghost_map.
 From iris.program_logic Require Import language.
 Require Import SailStdpp.Operators_mwords.
 Require Import Riscv.rv64d_types Riscv.rv64d Riscv.riscv_extras.
+Require Import WpGprCsrwCommon.
 Require Import RiscvModelBytes.
 Require Import SailStdpp.Base SailStdpp.TypeCasts.
 Require Import RiscvLang RiscvPtsto RiscvExec RiscvTryStep RiscvFetchExec RiscvExtras WpDecode WpLeafCommon WpGpr.
